Low-level parsers and serializers for Integers

src/lowparse/LowParse.Low.Int.Aux.fst
@@ -10,7 +10,7 @@ module U32 = FStar.UInt32
 module B = LowStar.Buffer
 
 inline_for_extraction
-let parse32_u16 : parser32 parse_u16 =
+let parse32_u16 : leaf_reader parse_u16 =
   decode_u16_injective ();
     make_total_constant_size_parser32 2 2ul
       #U16.t
@@ -20,7 +20,7 @@ let parse32_u16 : parser32 parse_u16 =
         E.be_to_n_2 _ _ (E.u16 ()) input)
 
 inline_for_extraction
-let parse32_u32 : parser32 parse_u32 =
+let parse32_u32 : leaf_reader parse_u32 =
     decode_u32_injective ();
     make_total_constant_size_parser32 4 4ul
       #U32.t
@@ -30,56 +30,30 @@ let parse32_u32 : parser32 parse_u32 =
         E.be_to_n_4 _ _ (E.u32 ()) input)
 
 inline_for_extraction
-let parse32_u8 : parser32 parse_u8 =
+let parse32_u8 : leaf_reader parse_u8 =
   decode_u8_injective ();
   make_total_constant_size_parser32 1 1ul
     decode_u8
     ()
     (fun b -> B.index b 0ul)
 
-module HST = FStar.HyperStack.ST
-
-#push-options "--z3rlimit 32"
+inline_for_extraction
+let serialize32_u8 : serializer32 #_ #_ #parse_u8 serialize_u8 =
+  fun v out ->
+  let out' = B.sub out 0ul 1ul in
+  B.upd out' 0ul v;
+  1ul
 
 inline_for_extraction
 let serialize32_u16 : serializer32 #_ #_ #parse_u16 serialize_u16 =
-  fun out lo v ->
-  assert (Seq.length (serialize #_ #_ #parse_u16 serialize_u16 v) == 2);
-  let out' = B.sub out lo 2ul in
-  assert_norm (pow2 (8 `Prims.op_Multiply` 2) == 65536);
-  let h = HST.get () in
-  assert (B.live h out'); 
-  assert (B.length out' == 2);
-  assert (8 `Prims.op_Multiply` 2 <= 16);
-  assert (U16.v v < pow2 (8 `Prims.op_Multiply` 2));
+  fun v out ->
+  let out' = B.sub out 0ul 2ul in
   E.n_to_be_2 U16.t 16 (E.u16 ()) v out';
-  let h' = HST.get () in
-  loc_jbuffer_eq out lo (U32.add lo 2ul);
-  exactly_contains_valid_data_equiv h' parse_u16 out lo v (U32.add lo 2ul)
+  2ul
 
-#pop-options
-
-inline_for_extraction
-let serialize32_u16_fail = serializer32_fail_of_serializer #_ #_ #parse_u16 #serialize_u16 serialize32_u16 2l
-
-#push-options "--z3rlimit 20"
 inline_for_extraction
 let serialize32_u32 : serializer32 #_ #_ #parse_u32 serialize_u32 =
-  fun out lo v ->
-  assert (Seq.length (serialize #_ #_ #parse_u32 serialize_u32 v) == 4);
-  let out' = B.sub out lo 4ul in
-  assert_norm (pow2 (8 `Prims.op_Multiply` 4) == 4294967296);
-  let h = HST.get () in
-  assert (B.live h out'); 
-  assert (B.length out' == 4);
-  assert (8 `Prims.op_Multiply` 4 <= 32);
-  assert (U32.v v <= pow2 32 - 1);
-  assert (U32.v v < pow2 (8 `Prims.op_Multiply` 4));
+  fun v out ->
+  let out' = B.sub out 0ul 4ul in
   E.n_to_be_4 U32.t 32 (E.u32 ()) v out';
-  let h' = HST.get () in
-  loc_jbuffer_eq out lo (U32.add lo 4ul);
-  exactly_contains_valid_data_equiv h' parse_u32 out lo v (U32.add lo 4ul)
-#pop-options
-
-inline_for_extraction
-let serialize32_u32_fail = serializer32_fail_of_serializer #_ #_ #parse_u32 #serialize_u32 serialize32_u32 4l
+  4ul
